ironfleet/src/Dafny/Distributed/Protocol/RSL/FailureProof/Phase2_PostFail/GenericLemmas.i.dfy
@@ -8,9 +8,9 @@ import opened RslPhase2Proof_PostFail_i
 
 /* There can be no 2b messages in the system before there are 2a's */
 lemma {:timeLimitMultiplier 2} lemma_NoNew2bBefore2aSent(ts:TimestampedRslState, ts':TimestampedRslState, op:OperationNumber, idx:int, tios:seq<TimestampedLIoOp<NodeIdentity, RslMessage>>) 
-    requires P2Assumption(ts, op) && RslConsistency(ts)
-    requires P2Assumption(ts', op) && RslConsistency(ts')
-    requires PacketsBallotInvariant(ts) && PacketsBallotInvariant(ts')
+    requires CommonAssumptions(ts) && CommonAssumptions(ts')
+    requires P2Assumption(ts, op)
+    requires PacketsBallotInvariant(ts)
     requires TimestampedRslNext(ts, ts')
     requires !TimestampedRslNextEnvironment(ts, ts')
     requires TimestampedRslNextOneReplica(ts, ts', idx, tios)
@@ -67,8 +67,8 @@ lemma {:timeLimitMultiplier 2} lemma_NoNew2bBefore2aSent(ts:TimestampedRslState,
 
 /* Non-leader replicas do not send 2a's */
 lemma lemma_NonLeaderDoesNotSend2a(ts:TimestampedRslState, ts':TimestampedRslState, op:OperationNumber, idx:int, tios:seq<TimestampedLIoOp<NodeIdentity, RslMessage>>) 
-    requires P2Assumption(ts, op) && RslConsistency(ts)
-    requires P2Assumption(ts', op) && RslConsistency(ts')
+    requires CommonAssumptions(ts) && CommonAssumptions(ts')
+    requires P2Assumption(ts, op)
     requires TimestampedRslNext(ts, ts')
     requires !TimestampedRslNextEnvironment(ts, ts')
     requires TimestampedRslNextOneReplica(ts, ts', idx, tios)
@@ -97,8 +97,8 @@ lemma lemma_NonLeaderDoesNotSend2a(ts:TimestampedRslState, ts':TimestampedRslSta
 
 /* Non-leader replicas do not send 2a's */
 lemma lemma_NonLeaderDoesNotSend2a_Undelivered(ts:TimestampedRslState, ts':TimestampedRslState, op:OperationNumber, idx:int, tios:seq<TimestampedLIoOp<NodeIdentity, RslMessage>>) 
-    requires P2Assumption(ts, op) && RslConsistency(ts)
-    requires P2Assumption(ts', op) && RslConsistency(ts')
+    requires CommonAssumptions(ts) && CommonAssumptions(ts')
+    requires P2Assumption(ts, op)
     requires TimestampedRslNext(ts, ts')
     requires !TimestampedRslNextEnvironment(ts, ts')
     requires TimestampedRslNextOneReplica(ts, ts', idx, tios)
@@ -126,8 +126,8 @@ lemma lemma_NonLeaderDoesNotSend2a_Undelivered(ts:TimestampedRslState, ts':Times
 
 /* Non-leader replicas do not send replies */
 lemma lemma_NonLeaderDoesNotSendReply(ts:TimestampedRslState, ts':TimestampedRslState, op:OperationNumber, idx:int, tios:seq<TimestampedLIoOp<NodeIdentity, RslMessage>>) 
-    requires P2Assumption(ts, op) && RslConsistency(ts)
-    requires P2Assumption(ts', op) && RslConsistency(ts')
+    requires CommonAssumptions(ts) && CommonAssumptions(ts')
+    requires P2Assumption(ts, op)
     requires TimestampedRslNext(ts, ts')
     requires !TimestampedRslNextEnvironment(ts, ts')
     requires TimestampedRslNextOneReplica(ts, ts', idx, tios)
@@ -157,8 +157,8 @@ lemma lemma_NonLeaderDoesNotSendReply(ts:TimestampedRslState, ts':TimestampedRsl
 
 /* Non-leader replicas do not send replies */
 lemma lemma_NonLeaderDoesNotSendReply_Undelivered(ts:TimestampedRslState, ts':TimestampedRslState, op:OperationNumber, idx:int, tios:seq<TimestampedLIoOp<NodeIdentity, RslMessage>>) 
-    requires P2Assumption(ts, op) && RslConsistency(ts)
-    requires P2Assumption(ts', op) && RslConsistency(ts')
+    requires CommonAssumptions(ts) && CommonAssumptions(ts')
+    requires P2Assumption(ts, op)
     requires TimestampedRslNext(ts, ts')
     requires !TimestampedRslNextEnvironment(ts, ts')
     requires TimestampedRslNextOneReplica(ts, ts', idx, tios)
@@ -184,41 +184,41 @@ lemma lemma_NonLeaderDoesNotSendReply_Undelivered(ts:TimestampedRslState, ts':Ti
     }
 }
 
-/* There can be no 1b messages sent in a Non-Receive step  */
-lemma lemma_No1bSentInNonReceiveStep(ts:TimestampedRslState, ts':TimestampedRslState, op:OperationNumber, idx:int, tios:seq<TimestampedLIoOp<NodeIdentity, RslMessage>>) 
-    requires P2Assumption(ts, op) && RslConsistency(ts)
-    requires P2Assumption(ts', op) && RslConsistency(ts')
-    requires TimestampedRslNext(ts, ts')
-    requires !TimestampedRslNextEnvironment(ts, ts')
-    requires TimestampedRslNextOneReplica(ts, ts', idx, tios)
-    requires Phase2Invariant(ts, op)
-    requires ts.t_replicas[idx].v.nextActionIndex != 0
-    // ensures forall pkt | pkt in ts'.t_environment.sentPackets && pkt.msg.v.RslMessage_2b? :: pkt in ts.t_environment.sentPackets
-    ensures forall pkt | pkt in ts'.undeliveredPackets && pkt.msg.v.RslMessage_1b? :: pkt in ts.undeliveredPackets
-{
-    var ls, ls' := ts.t_replicas[idx], ts'.t_replicas[idx];
-    var nextActionIndex := ls.v.nextActionIndex;
-    forall pkt | pkt in ts'.t_environment.sentPackets && pkt.msg.v.RslMessage_1b?
-    ensures pkt in ts.t_environment.sentPackets 
-    {
-        if pkt !in ts.t_environment.sentPackets {
-            var ios := UntagLIoOpSeq(tios);
-            var sent_packets := ExtractSentPacketsFromIos(ios);
-            assert LReplicaNoReceiveNext(ls.v.replica, nextActionIndex, ls'.v.replica, ios);
-            assert forall p | p in sent_packets :: !p.msg.RslMessage_1b?;
-            forall io | io in tios && io.LIoOpSend?
-            ensures !io.s.msg.v.RslMessage_1b? {}
-            assert false;
-        }
-    }
-    lemma_No2bSentInNonReceiveStep_Undelivered(ts, ts', op, idx, tios);
-}
+// /* There can be no 1b messages sent in a Non-Receive step  */
+// lemma lemma_No1bSentInNonReceiveStep(ts:TimestampedRslState, ts':TimestampedRslState, op:OperationNumber, idx:int, tios:seq<TimestampedLIoOp<NodeIdentity, RslMessage>>) 
+//     requires P2Assumption(ts, op) && RslConsistency(ts)
+//     requires P2Assumption(ts', op) && RslConsistency(ts')
+//     requires TimestampedRslNext(ts, ts')
+//     requires !TimestampedRslNextEnvironment(ts, ts')
+//     requires TimestampedRslNextOneReplica(ts, ts', idx, tios)
+//     requires Phase2Invariant(ts, op)
+//     requires ts.t_replicas[idx].v.nextActionIndex != 0
+//     // ensures forall pkt | pkt in ts'.t_environment.sentPackets && pkt.msg.v.RslMessage_2b? :: pkt in ts.t_environment.sentPackets
+//     ensures forall pkt | pkt in ts'.undeliveredPackets && pkt.msg.v.RslMessage_1b? :: pkt in ts.undeliveredPackets
+// {
+//     var ls, ls' := ts.t_replicas[idx], ts'.t_replicas[idx];
+//     var nextActionIndex := ls.v.nextActionIndex;
+//     forall pkt | pkt in ts'.t_environment.sentPackets && pkt.msg.v.RslMessage_1b?
+//     ensures pkt in ts.t_environment.sentPackets 
+//     {
+//         if pkt !in ts.t_environment.sentPackets {
+//             var ios := UntagLIoOpSeq(tios);
+//             var sent_packets := ExtractSentPacketsFromIos(ios);
+//             assert LReplicaNoReceiveNext(ls.v.replica, nextActionIndex, ls'.v.replica, ios);
+//             assert forall p | p in sent_packets :: !p.msg.RslMessage_1b?;
+//             forall io | io in tios && io.LIoOpSend?
+//             ensures !io.s.msg.v.RslMessage_1b? {}
+//             assert false;
+//         }
+//     }
+//     lemma_No2bSentInNonReceiveStep_Undelivered(ts, ts', op, idx, tios);
+// }
 
 
 /* There can be no 2b messages sent in a Non-Receive step  */
 lemma lemma_No2bSentInNonReceiveStep(ts:TimestampedRslState, ts':TimestampedRslState, op:OperationNumber, idx:int, tios:seq<TimestampedLIoOp<NodeIdentity, RslMessage>>) 
-    requires P2Assumption(ts, op) && RslConsistency(ts)
-    requires P2Assumption(ts', op) && RslConsistency(ts')
+    requires CommonAssumptions(ts) && CommonAssumptions(ts')
+    requires P2Assumption(ts, op)
     requires TimestampedRslNext(ts, ts')
     requires !TimestampedRslNextEnvironment(ts, ts')
     requires TimestampedRslNextOneReplica(ts, ts', idx, tios)
@@ -247,8 +247,8 @@ lemma lemma_No2bSentInNonReceiveStep(ts:TimestampedRslState, ts':TimestampedRslS
 
 
 lemma lemma_No2bSentInNonReceiveStep_Undelivered(ts:TimestampedRslState, ts':TimestampedRslState, op:OperationNumber, idx:int, tios:seq<TimestampedLIoOp<NodeIdentity, RslMessage>>) 
-    requires P2Assumption(ts, op) && RslConsistency(ts)
-    requires P2Assumption(ts', op) && RslConsistency(ts')
+    requires CommonAssumptions(ts) && CommonAssumptions(ts')
+    requires P2Assumption(ts, op)
     requires TimestampedRslNext(ts, ts')
     requires !TimestampedRslNextEnvironment(ts, ts')
     requires TimestampedRslNextOneReplica(ts, ts', idx, tios)
@@ -274,73 +274,73 @@ lemma lemma_No2bSentInNonReceiveStep_Undelivered(ts:TimestampedRslState, ts':Tim
 }
 
 
-/* There can be no 2b messages sent in a receive step unless receiving 2a  */
-lemma lemma_No2bSentInReceiveStep_NotReceive2a(ts:TimestampedRslState, ts':TimestampedRslState, op:OperationNumber, idx:int, tios:seq<TimestampedLIoOp<NodeIdentity, RslMessage>>) 
-    requires P2Assumption(ts, op) && RslConsistency(ts)
-    requires P2Assumption(ts', op) && RslConsistency(ts')
-    requires TimestampedRslNext(ts, ts')
-    requires !TimestampedRslNextEnvironment(ts, ts')
-    requires TimestampedRslNextOneReplica(ts, ts', idx, tios)
-    requires Phase2Invariant(ts, op)
-    requires ts.t_replicas[idx].v.nextActionIndex == 0
-    requires !tios[0].r.msg.v.RslMessage_2a? 
-    ensures forall pkt | pkt in ts'.t_environment.sentPackets && pkt.msg.v.RslMessage_2b? :: pkt in ts.t_environment.sentPackets
-    ensures forall pkt | pkt in ts'.undeliveredPackets && pkt.msg.v.RslMessage_2b? :: pkt in ts.undeliveredPackets
-{
-    var ls, ls' := ts.t_replicas[idx], ts'.t_replicas[idx];
-    forall p | p in ts'.t_environment.sentPackets && p.msg.v.RslMessage_2b? 
-    ensures p in ts.t_environment.sentPackets
-    {
-        if p !in ts.t_environment.sentPackets {
-            var sent_packets := ExtractSentPacketsFromIos(UntagLIoOpSeq(tios));
-            forall p | p in sent_packets 
-            ensures !p.msg.RslMessage_2b? {}
-            assert false;
-        }
-    }
-    forall p | p in ts'.undeliveredPackets && p.msg.v.RslMessage_2b?
-    ensures p in ts.undeliveredPackets
-    {
-        if p !in ts.t_environment.sentPackets {
-            var sent_packets := ExtractSentPacketsFromIos(UntagLIoOpSeq(tios));
-            forall p | p in sent_packets 
-            ensures !p.msg.RslMessage_2b? {}
-            assert false;
-        }
-    }
-}
+// /* There can be no 2b messages sent in a receive step unless receiving 2a  */
+// lemma lemma_No2bSentInReceiveStep_NotReceive2a(ts:TimestampedRslState, ts':TimestampedRslState, op:OperationNumber, idx:int, tios:seq<TimestampedLIoOp<NodeIdentity, RslMessage>>) 
+//     requires P2Assumption(ts, op) && RslConsistency(ts)
+//     requires P2Assumption(ts', op) && RslConsistency(ts')
+//     requires TimestampedRslNext(ts, ts')
+//     requires !TimestampedRslNextEnvironment(ts, ts')
+//     requires TimestampedRslNextOneReplica(ts, ts', idx, tios)
+//     requires Phase2Invariant(ts, op)
+//     requires ts.t_replicas[idx].v.nextActionIndex == 0
+//     requires !tios[0].r.msg.v.RslMessage_2a? 
+//     ensures forall pkt | pkt in ts'.t_environment.sentPackets && pkt.msg.v.RslMessage_2b? :: pkt in ts.t_environment.sentPackets
+//     ensures forall pkt | pkt in ts'.undeliveredPackets && pkt.msg.v.RslMessage_2b? :: pkt in ts.undeliveredPackets
+// {
+//     var ls, ls' := ts.t_replicas[idx], ts'.t_replicas[idx];
+//     forall p | p in ts'.t_environment.sentPackets && p.msg.v.RslMessage_2b? 
+//     ensures p in ts.t_environment.sentPackets
+//     {
+//         if p !in ts.t_environment.sentPackets {
+//             var sent_packets := ExtractSentPacketsFromIos(UntagLIoOpSeq(tios));
+//             forall p | p in sent_packets 
+//             ensures !p.msg.RslMessage_2b? {}
+//             assert false;
+//         }
+//     }
+//     forall p | p in ts'.undeliveredPackets && p.msg.v.RslMessage_2b?
+//     ensures p in ts.undeliveredPackets
+//     {
+//         if p !in ts.t_environment.sentPackets {
+//             var sent_packets := ExtractSentPacketsFromIos(UntagLIoOpSeq(tios));
+//             forall p | p in sent_packets 
+//             ensures !p.msg.RslMessage_2b? {}
+//             assert false;
+//         }
+//     }
+// }
 
 
-lemma lemma_No1bSentInReceiveStep_NotReceive1a(ts:TimestampedRslState, ts':TimestampedRslState, op:OperationNumber, idx:int, tios:seq<TimestampedLIoOp<NodeIdentity, RslMessage>>) 
-    requires P2Assumption(ts, op) && RslConsistency(ts)
-    requires P2Assumption(ts', op) && RslConsistency(ts')
-    requires TimestampedRslNext(ts, ts')
-    requires !TimestampedRslNextEnvironment(ts, ts')
-    requires TimestampedRslNextOneReplica(ts, ts', idx, tios)
-    requires Phase2Invariant(ts, op)
-    requires ts.t_replicas[idx].v.nextActionIndex == 0
-    requires !tios[0].r.msg.v.RslMessage_1a? 
-    // ensures forall pkt | pkt in ts'.t_environment.sentPackets && pkt.msg.v.RslMessage_2b? :: pkt in ts.t_environment.sentPackets
-    ensures forall pkt | pkt in ts'.undeliveredPackets && pkt.msg.v.RslMessage_1b? :: pkt in ts.undeliveredPackets
-{
-    var ls, ls' := ts.t_replicas[idx], ts'.t_replicas[idx];
-    forall p | p in ts'.undeliveredPackets && p.msg.v.RslMessage_1b?
-    ensures p in ts.undeliveredPackets
-    {
-        if p !in ts.t_environment.sentPackets {
-            var sent_packets := ExtractSentPacketsFromIos(UntagLIoOpSeq(tios));
-            forall p | p in sent_packets 
-            ensures !p.msg.RslMessage_1b? {}
-            assert false;
-        }
-    }
-}
+// lemma lemma_No1bSentInReceiveStep_NotReceive1a(ts:TimestampedRslState, ts':TimestampedRslState, op:OperationNumber, idx:int, tios:seq<TimestampedLIoOp<NodeIdentity, RslMessage>>) 
+//     requires P2Assumption(ts, op) && RslConsistency(ts)
+//     requires P2Assumption(ts', op) && RslConsistency(ts')
+//     requires TimestampedRslNext(ts, ts')
+//     requires !TimestampedRslNextEnvironment(ts, ts')
+//     requires TimestampedRslNextOneReplica(ts, ts', idx, tios)
+//     requires Phase2Invariant(ts, op)
+//     requires ts.t_replicas[idx].v.nextActionIndex == 0
+//     requires !tios[0].r.msg.v.RslMessage_1a? 
+//     // ensures forall pkt | pkt in ts'.t_environment.sentPackets && pkt.msg.v.RslMessage_2b? :: pkt in ts.t_environment.sentPackets
+//     ensures forall pkt | pkt in ts'.undeliveredPackets && pkt.msg.v.RslMessage_1b? :: pkt in ts.undeliveredPackets
+// {
+//     var ls, ls' := ts.t_replicas[idx], ts'.t_replicas[idx];
+//     forall p | p in ts'.undeliveredPackets && p.msg.v.RslMessage_1b?
+//     ensures p in ts.undeliveredPackets
+//     {
+//         if p !in ts.t_environment.sentPackets {
+//             var sent_packets := ExtractSentPacketsFromIos(UntagLIoOpSeq(tios));
+//             forall p | p in sent_packets 
+//             ensures !p.msg.RslMessage_1b? {}
+//             assert false;
+//         }
+//     }
+// }
 
 
 /* There can be no 2a messages sent in a Receive step  */
 lemma {:timeLimitMultiplier 2} lemma_No2aSentInNon2aStep(ts:TimestampedRslState, ts':TimestampedRslState, op:OperationNumber, idx:int, tios:seq<TimestampedLIoOp<NodeIdentity, RslMessage>>) 
-    requires P2Assumption(ts, op) && RslConsistency(ts)
-    requires P2Assumption(ts', op) && RslConsistency(ts')
+    requires CommonAssumptions(ts) && CommonAssumptions(ts')
+    requires P2Assumption(ts, op)
     requires TimestampedRslNext(ts, ts')
     requires !TimestampedRslNextEnvironment(ts, ts')
     requires TimestampedRslNextOneReplica(ts, ts', idx, tios)
@@ -381,8 +381,8 @@ lemma {:timeLimitMultiplier 2} lemma_No2aSentInNon2aStep(ts:TimestampedRslState,
 
 /* There can be no Reply messages sent in a Non-Execution step  */
 lemma lemma_NoRepliesSentInNonExecutionStep(ts:TimestampedRslState, ts':TimestampedRslState, op:OperationNumber, idx:int, tios:seq<TimestampedLIoOp<NodeIdentity, RslMessage>>) 
-    requires P2Assumption(ts, op) && RslConsistency(ts)
-    requires P2Assumption(ts', op) && RslConsistency(ts')
+    requires CommonAssumptions(ts) && CommonAssumptions(ts')
+    requires P2Assumption(ts, op)
     requires TimestampedRslNext(ts, ts')
     requires !TimestampedRslNextEnvironment(ts, ts')
     requires TimestampedRslNextOneReplica(ts, ts', idx, tios)
@@ -394,8 +394,8 @@ lemma lemma_NoRepliesSentInNonExecutionStep(ts:TimestampedRslState, ts':Timestam
 
 /* In a receive step, if sent_packets is empty, no packets get added to the network */
 lemma lemma_EmptySentPackets(ts:TimestampedRslState, ts':TimestampedRslState, op:OperationNumber, idx:int, tios:seq<TimestampedLIoOp<NodeIdentity, RslMessage>>) 
-    requires P2Assumption(ts, op) && RslConsistency(ts)
-    requires P2Assumption(ts', op) && RslConsistency(ts')
+    requires CommonAssumptions(ts) && CommonAssumptions(ts')
+    requires P2Assumption(ts, op)
     requires TimestampedRslNext(ts, ts')
     requires !TimestampedRslNextEnvironment(ts, ts')
     requires TimestampedRslNextOneReplica(ts, ts', idx, tios)
